theories/L2_typeStripped/wcbvEval.v
@@ -27,7 +27,7 @@ Inductive WcbvEval (p:environ Term) : Term -> Term -> Prop :=
 | wInd: forall i, WcbvEval p (TInd i) (TInd i) 
 | wSort: forall srt, WcbvEval p (TSort srt) (TSort srt)
 | wFix: forall dts m, WcbvEval p (TFix dts m) (TFix dts m)
-| wAx: WcbvEval p TAx TAx
+| wAx: forall s, WcbvEval p (TAx s) (TAx s)
 | wConst: forall nm (t s:Term),
             lookupDfn nm p = Ret t -> WcbvEval p t s ->
             WcbvEval p (TConst nm) s
@@ -40,26 +40,16 @@ Inductive WcbvEval (p:environ Term) : Term -> Term -> Prop :=
             WcbvEval p dfn dfn' ->
             WcbvEval p (instantiate dfn' 0 bod) s ->
             WcbvEval p (TLetIn nm dfn bod) s
-| wAppFix: forall dts m (fn arg arg' s x:Term)
-                  (args args':Terms) (ix:nat),
+| wAppFix: forall dts m (fn arg s x:Term) (args:Terms) (ix:nat),
              WcbvEval p fn (TFix dts m) ->
-             WcbvEvals p (tcons arg args) (tcons arg' args') ->
              dnthBody m dts = Some (x, ix) ->
-             ix <= tlength args ->     (* enough args *)
-             WcbvEval p (pre_whFixStep x dts (tcons arg' args')) s ->
+             WcbvEval p (pre_whFixStep x dts (tcons arg args)) s ->
              WcbvEval p (TApp fn arg args) s 
 | wAppCong: forall fn fn' arg args aargs',
               WcbvEval p fn fn' ->
               ~ isLambda fn' -> ~ isFix fn' ->
               WcbvEvals p (tcons arg args) aargs' ->
               WcbvEval p (TApp fn arg args) (mkApp fn' aargs')
-| wAppFixCong1: forall dts m (fn arg arg' x:Term)
-                  (args args':Terms) (ix:nat),
-             WcbvEval p fn (TFix dts m) ->
-             WcbvEvals p (tcons arg args) (tcons arg' args') ->
-             dnthBody m dts = Some (x, ix) ->
-             ix > tlength args ->     (* too few args *)
-             WcbvEval p (TApp fn arg args) (TApp (TFix dts m) arg' args')
 | wCase: forall mch Mch n args ml ts brs cs s ,
                 WcbvEval p mch Mch ->
                 canonicalP Mch = Some (n, args) ->
@@ -159,10 +149,8 @@ Proof.
     specialize (H H4). inversion_Clear H.
     apply (whBetaStep_pres_WFapp); intuition. 
   - inversion_Clear H1. apply H0. apply instantiate_pres_WFapp; intuition.
-  - inversion_clear H2. specialize (H H4). inversion_Clear H.
-    assert (j: WFapps (tcons arg args)).
-    { constructor; assumption. }
-    apply H1. apply pre_whFixStep_pres_WFapp; try eassumption; intuition.
+  - inversion_clear H1. specialize (H H3). inversion_Clear H.
+    apply H0. apply pre_whFixStep_pres_WFapp; try eassumption; intuition.
     + eapply dnthBody_pres_WFapp; try eassumption.
   - inversion_Clear H1.
     destruct (WcbvEvals_tcons_tcons w0) as [x0 [x1 jx]]. subst.    
@@ -179,10 +167,6 @@ Proof.
       rewrite <- k. constructor; try assumption.
       rewrite <- tappend_assoc. cbn. apply tappend_pres_WFapps; try assumption.
       apply H0. constructor; try assumption.
-  - inversion_Clear H1. specialize (H H6).
-    assert (k: WFapps (tcons arg args)). intuition.
-    specialize (H0 k). inversion_Clear H0.
-    constructor; try assumption. not_isApp.
   - apply H0. inversion_Clear H1. 
     refine (whCaseStep_pres_WFapp H6 _ _ e1). 
     refine (tskipn_pres_WFapp _ _ e0).
@@ -216,7 +200,6 @@ Proof.
     + apply H1. assumption.
   - eapply wLetIn; intuition.
   - eapply wAppFix; try eassumption; intuition. 
-  - eapply wAppFixCong1; try eassumption; intuition.    
   - eapply wCase; intuition; eassumption.
 Qed.
 
@@ -358,7 +341,7 @@ Proof.
     + eapply wERTCtrn. apply wERTCstep. apply sLetIn. apply H0.
       apply instantiate_pres_WFapp; try assumption.
       * eapply (proj1 (WcbvEval_pres_WFapp hp)); try eassumption.
-  - inversion_clear H2. specialize (H H4).
+ - inversion_clear H1. specialize (H H3).
     assert (j0: WFapps (tcons arg args)).
     { constructor; assumption. }
     assert (j2: WFapp (TFix dts m)).
@@ -366,23 +349,16 @@ Proof.
     inversion_clear j2.
     assert (j3: WFapp x).
     { refine (dnthBody_pres_WFapp _ _ e). assumption. }
-    specialize (H0 j0).
-    assert (j4: WFapp (pre_whFixStep x dts (tcons arg' args'))).
-    { refine (pre_whFixStep_pres_WFapp _ _ _); try assumption.
-      eapply (proj2 (WcbvEval_pres_WFapp hp)); eassumption. }
-    specialize (H1 j4).
+    assert (j4: WFapp (pre_whFixStep x dts (tcons arg args))).
+    { refine (pre_whFixStep_pres_WFapp _ _ _); try assumption. }
+    specialize (H0 j4).
     refine (@wERTCtrn _ _ (TApp (TFix dts m) arg args) _ _ _).
     + rewrite <- mkApp_goodFn; try assumption.
       rewrite <- mkApp_goodFn; try not_isApp.
       apply wndEvalRTC_App_fn; assumption.
-    + eapply (@wERTCtrn _ _ (TApp (TFix dts m) arg' args')).
-      eapply (wndEvalsRTC_App_args); try reflexivity; try eassumption.
-      * not_isApp.
-      * { eapply (@wERTCtrn _ _  (pre_whFixStep x dts (tcons arg' args'))).
-          - eapply wERTCstep. eapply sFix; try eassumption.
-            inversion_clear w0.
-            erewrite <- WcbvEvals_pres_tlength; try eassumption.
-          - assumption. }
+    + eapply (@wERTCtrn _ _  (pre_whFixStep x dts (tcons arg args))).
+      * eapply wERTCstep. eapply sFix; try eassumption.
+      * assumption.
   - inversion_Clear H1. specialize (H H6). specialize (H0 (wfacons H7 H8)).
     destruct (WcbvEvals_tcons_tcons w0) as [x0 [x1 jx]]. subst.
     eapply (@wERTCtrn _ _ (TApp fn x0 x1)).
@@ -393,22 +369,6 @@ Proof.
         constructor; assumption. }
       inversion_Clear j.
       eapply wndEvalRTC_App_fn; try assumption.
-  - inversion_Clear H1. specialize (H H6).
-    assert (k: WFapps (tcons arg args)). intuition.
-    specialize (H0 k).
-    eapply (@wERTCtrn _ _ (TApp (TFix dts m) arg args)).
-    + rewrite <- mkApp_goodFn; try assumption.
-      rewrite <- mkApp_goodFn; try not_isApp.
-      apply wndEvalRTC_App_fn; assumption.
-    + eapply (@wERTCtrn _ _ (mkApp (TFix dts m) (tcons arg' args'))).
-      * rewrite mkApp_goodFn.
-        eapply wndEvalsRTC_App_args; try reflexivity; try assumption.
-        not_isApp. not_isApp.
-      * { eapply (@wERTCtrn _ _ (TApp (TFix dts m) arg' args')).
-          - eapply wndEvalsRTC_App_args; try reflexivity.
-            + apply wndEvalsRTC_mk_tconsr; try assumption. constructor.
-            + not_isApp.
-          - constructor. }
   - inversion_Clear H1. eapply wERTCtrn. 
     + eapply wndEvalRTC_Case_mch. apply H. assumption.
     + eapply (@wERTCtrn _ _ cs). 
@@ -456,103 +416,93 @@ Variable p:environ Term.
 Function wcbvEval
          (tmr:nat) (t:Term) {struct tmr}: exception Term :=
   match tmr with 
-    | 0 => raise ("out of time: " ++ print_term t)
-    | S n =>
-      match t with      (** look for a redex **)
-        | TConst nm =>
-          match (lookup nm p) with
-            | Some (ecTrm t) => wcbvEval n t
-                  (** note hack coding of axioms in environment **)
-            | Some (ecTyp _ _ _) => raise ("wcbvEval, TConst ecTyp " ++ nm)
-            | _ => raise "wcbvEval: TConst environment miss"
-          end
-        | TCast t =>
-          match wcbvEval n t with
-            | Ret et => Ret et
-            | Exc s => raise ("wcbvEval: TCast: " ++ s)
-          end
-        | TProof t =>
-          match wcbvEval n t with
-            | Ret et => Ret et
-            | Exc s => raise ("wcbvEval: TProof: " ++ s)
-          end
-        | TApp fn a1 args =>
-          match wcbvEval n fn with
-            | Exc s => raise ("wcbvEval TApp: fn doesn't eval: " ++ s)
-            | Ret (TLambda _ bod) =>
-              match wcbvEval n a1 with
-                | Exc s =>  raise ("wcbvEval TApp: arg doesn't eval: " ++ s)
-                | Ret b1 => wcbvEval n (whBetaStep bod b1 args)
-              end
-            | Ret (TFix dts m) =>           (* Fix redex *)
-              match dnthBody m dts with
-                | None => raise ("wcbvEval TApp: dnthBody doesn't eval: ")
-                | Some (x, ix) =>
-                  match wcbvEvals n (tcons a1 args) with
-                    | Ret (tcons arg' args') =>
-                      match le_lt_dec ix (tlength args) with
-                        | left _ _ =>
-                          wcbvEval n (pre_whFixStep x dts (tcons arg' args'))
-                        | right _ _ =>  ret (TApp (TFix dts m) arg' args')
-                      end
-                    | Ret tnil => raise ("wcbvEval TAppFix: args nil")
-                    | Exc s => raise ("wcbvEval TAppFix: args " ++ s)
-                  end
-              end
-            | Ret Fn =>              (* no redex; congruence rule *)
-              match wcbvEvals n (tcons a1 args) with
-                | Exc s => raise ("wcbvEval TApp: args don't eval: " ++ s)
-                | Ret ergs => ret (mkApp Fn ergs)
-              end
-          end
-        | TCase ml mch brs =>
-          match wcbvEval n mch with
-            | Exc str => Exc str
-            | Ret emch =>
-              match canonicalP emch with
-                | None => Ret (TCase ml emch brs)
-                | Some (r, args) =>
-                  match tskipn (snd ml) args with
-                    | None => raise "wcbvEval: Case, tskipn"
-                    | Some ts =>
-                      match whCaseStep r ts brs with
-                        | None => raise "wcbvEval: Case, whCaseStep"
-                        | Some cs => wcbvEval n cs
-                      end
-                  end
-              end
-          end
-        | TLetIn nm df bod =>
-          match wcbvEval n df with
-            | Ret df' => wcbvEval n (instantiate df' 0 bod)
-            | Exc s => raise ("wcbvEval: TLetIn: " ++ s)
-          end
-        (** already in whnf ***)
-        | TAx => ret TAx
-        | TLambda nn t => ret (TLambda nn t)
-        | TProd nn t => ret (TProd nn t)
-        | TFix mfp br => ret (TFix mfp br)
-        | TConstruct i cn np na => ret (TConstruct i cn np na)
-        | TInd i => ret (TInd i)
-        | TSort srt => ret (TSort srt)
-        (** should never appear **)
-        | TRel _ => raise "wcbvEval: unbound Rel"
-        | TWrong => ret TWrong
+  | 0 => raise ("out of time: " ++ print_term t)
+  | S n =>
+    match t with      (** look for a redex **)
+    | TConst nm =>
+      match (lookup nm p) with
+      | Some (ecTrm t) => wcbvEval n t
+      (** note hack coding of axioms in environment **)
+      | Some (ecTyp _ _ _) => raise ("wcbvEval, TConst ecTyp " ++ nm)
+      | _ => raise "wcbvEval: TConst environment miss"
       end
+    | TCast t =>
+      match wcbvEval n t with
+      | Ret et => Ret et
+      | Exc s => raise ("wcbvEval: TCast: " ++ s)
+      end
+    | TProof t =>
+      match wcbvEval n t with
+      | Ret et => Ret et
+      | Exc s => raise ("wcbvEval: TProof: " ++ s)
+      end
+    | TApp fn a1 args =>
+      match wcbvEval n fn with
+      | Exc s => raise ("wcbvEval TApp: fn doesn't eval: " ++ s)
+      | Ret (TLambda _ bod) =>
+        match wcbvEval n a1 with
+        | Exc s =>  raise ("wcbvEval TApp: arg doesn't eval: " ++ s)
+        | Ret b1 => wcbvEval n (whBetaStep bod b1 args)
+        end
+      | Ret (TFix dts m) =>           (* Fix redex *)
+        match dnthBody m dts with
+        | None => raise ("wcbvEval TApp: dnthBody doesn't eval: ")
+        | Some (x, ix) => wcbvEval n (pre_whFixStep x dts (tcons a1 args))
+        end
+      | Ret Fn =>              (* no redex; congruence rule *)
+        match wcbvEvals n (tcons a1 args) with
+        | Exc s => raise ("wcbvEval TApp: args don't eval: " ++ s)
+        | Ret ergs => ret (mkApp Fn ergs)
+        end
+      end
+    | TCase ml mch brs =>
+      match wcbvEval n mch with
+      | Exc str => Exc str
+      | Ret emch =>
+        match canonicalP emch with
+        | None => Ret (TCase ml emch brs)
+        | Some (r, args) =>
+          match tskipn (snd ml) args with
+          | None => raise "wcbvEval: Case, tskipn"
+          | Some ts =>
+            match whCaseStep r ts brs with
+            | None => raise "wcbvEval: Case, whCaseStep"
+            | Some cs => wcbvEval n cs
+            end
+          end
+        end
+      end
+    | TLetIn nm df bod =>
+      match wcbvEval n df with
+      | Ret df' => wcbvEval n (instantiate df' 0 bod)
+      | Exc s => raise ("wcbvEval: TLetIn: " ++ s)
+      end
+    (** already in whnf ***)
+    | TAx s => ret (TAx s)
+    | TLambda nn t => ret (TLambda nn t)
+    | TProd nn t => ret (TProd nn t)
+    | TFix mfp br => ret (TFix mfp br)
+    | TConstruct i cn np na => ret (TConstruct i cn np na)
+    | TInd i => ret (TInd i)
+    | TSort srt => ret (TSort srt)
+    (** should never appear **)
+    | TRel _ => raise "wcbvEval: unbound Rel"
+    | TWrong => ret TWrong
+    end
   end
 with wcbvEvals (tmr:nat) (ts:Terms) {struct tmr}
      : exception Terms :=
        (match tmr with 
-          | 0 => raise "out of time"
-          | S n => match ts with             (** look for a redex **)
-                     | tnil => ret tnil
-                     | tcons s ss =>
-                       match wcbvEval n s, wcbvEvals n ss with
-                         | Ret es, Ret ess => ret (tcons es ess)
-                         | Exc s, _ => raise s
-                         | Ret _, Exc s => raise s
-                       end
+        | 0 => raise "out of time"
+        | S n => match ts with             (** look for a redex **)
+                 | tnil => ret tnil
+                 | tcons s ss =>
+                   match wcbvEval n s, wcbvEvals n ss with
+                   | Ret es, Ret ess => ret (tcons es ess)
+                   | Exc s, _ => raise s
+                   | Ret _, Exc s => raise s
                    end
+                 end
         end).
 Functional Scheme wcbvEval_ind' := Induction for wcbvEval Sort Prop
 with wcbvEvals_ind' := Induction for wcbvEvals Sort Prop.
@@ -574,10 +524,8 @@ Proof.
     + unfold lookupDfn. rewrite e1. reflexivity.
   - specialize (H1 _ p1). specialize (H _ e1). specialize (H0 _ e2).
     eapply wAppLam; eassumption.
-  - specialize (H1 _ p1). specialize (H _ e1). specialize (H0 _ e3).
+  - specialize (H0 _ p1). specialize (H _ e1).
     eapply wAppFix; try eassumption.
-  - specialize (H _ e1). specialize (H0 _ e3).
-    eapply wAppFixCong1; try eassumption.
   - specialize (H _ e1). specialize (H0 _ e2).
     eapply wAppCong; try eassumption.
     + destruct Fn; try not_isLambda. auto.
@@ -643,20 +591,10 @@ Lemma pre_WcbvEval_wcbvEval:
     assert (l1:= max_fst x x0). assert (l2:= max_snd x x0).
     simpl. rewrite (j mx x); try omega. rewrite (H (mx - 1)); try omega.
     rewrite H0; try omega. reflexivity.
- - destruct H, H0, H1. exists (S (max x0 (max x1 x2))). intros mx h.
-    assert (j1:= max_fst x0 (max x1 x2)). 
-    assert (lx: mx > x0). omega.
-    assert (j2:= max_snd x0 (max x1 x2)).
-    assert (j3:= max_fst x1 x2).
-    assert (lx0: mx > x1). omega.
-    assert (j4:= max_snd x1 x2).
-    assert (j5:= max_fst x1 x2).
-    assert (lx1: mx > x2). omega.
-    simpl. rewrite (j mx x0); try omega. rewrite H; try omega.
-    rewrite e. rewrite H0; try omega.
-    destruct (le_lt_dec ix (tlength args)).
-    + rewrite H1; try omega. reflexivity.
-    + omega.
+  - destruct H, H0. exists (S (max x0 x1)). intros mx h.
+    assert (l1:= max_fst x0 x1). assert (l2:= max_snd x0 x1).
+    cbn. rewrite (j mx x0); try omega. rewrite (H (mx - 1)); try omega.
+    rewrite e. rewrite H0; try omega. reflexivity.
   - destruct H, H0. exists (S (max x x0)). intros mx h.
     assert (l1:= max_fst x x0). assert (l2:= max_snd x x0).
     simpl. rewrite (j mx x); try omega. rewrite (H (mx - 1)); try omega.
@@ -664,12 +602,6 @@ Lemma pre_WcbvEval_wcbvEval:
     destruct fn'; try reflexivity.
     + elim n; auto.
     + elim n0; auto.
-  - destruct H, H0. exists (S (max x1 x0)). intros mx h.
-    assert (l1:= max_fst x1 x0). assert (l2:= max_snd x1 x0).
-    simpl. rewrite (j mx x1); try omega. rewrite (H (mx - 1)); try omega.
-    rewrite e. rewrite H0; try omega. destruct (le_lt_dec ix (tlength args)).
-    + omega.
-    + reflexivity.
   - destruct H, H0. exists (S (max x x0)). intros mx h.
     assert (l1:= max_fst x x0). assert (l2:= max_snd x x0).
     cbn. rewrite (j mx x); try omega. rewrite (H (mx - 1)); try omega.
