theories/L1g/wNorm.v
@@ -30,7 +30,7 @@ Inductive WNorm: Term -> Prop :=
 | WNLam: forall nm ty bod, WNorm ty -> WNorm (TLambda nm ty bod)
 | WNProd: forall nm ty bod, WNorm ty -> WNorm (TProd nm ty bod)
 | WNFix: forall ds br, WNorm (TFix ds br)
-| WNAx: WNorm TAx
+| WNAx: forall t, WNorm (TAx t)
 | WNCase: forall mch n ty brs,
             WNorm mch -> WNorm ty -> ~ isCanonical mch ->
             WNorm (TCase n ty mch brs)
@@ -41,11 +41,6 @@ Inductive WNorm: Term -> Prop :=
            WNorm fn -> WNorms (tcons t ts) ->
            ~ isLambda fn -> ~ isFix fn -> ~ isApp fn ->
            WNorm (TApp fn t ts)
-| WNAppFix: forall ds m t ts x ix,
-              WNorms (tcons t ts) ->
-              dnthBody m ds = Some (x, ix) ->
-              ix > tlength ts ->  (* too few args to see rec arg *)
-              WNorm (TApp (TFix ds m) t ts)
 with WNorms: Terms -> Prop :=
 | WNtnil: WNorms tnil
 | WNtcons: forall t ts, WNorm t -> WNorms ts -> WNorms (tcons t ts).
@@ -262,10 +257,6 @@ Proof.
     eapply canonicalP_isCanonical. eassumption.
   - inversion_Clear h.
     + elim H5. auto.
-    + rewrite e in H4. myInjection H4. omega.
-  - inversion_Clear h.
-    + contradiction.
-    + elim H. constructor.
 Qed.
 
 Lemma wNorm_no_wndStep:
